\documentclass[12pt]{article}

\usepackage[a4paper,top=1in,bottom=1in,left=1in,right=1in]{geometry}

\usepackage[utf8]{inputenc}
\usepackage{float}
\usepackage{amsmath}
\usepackage{graphicx}
\usepackage{titlesec}
\usepackage{tcolorbox}
\usepackage{enumitem}
\usepackage{tikz}
\usetikzlibrary{graphs}
\usetikzlibrary{graphdrawing}
\usegdlibrary{force}
\usepackage{amssymb}
\usepackage{hyperref}

\title{\bfseries Laborator Proiectare Logică 4}
\author{Sîrghe Matei}
\date{October 23, 2024}

\titleformat{\section}
  {\normalfont\Large\bfseries}{\thesection}{1em}{}
\begin{document}
\maketitle

Website: \href{https://lg.ccpr.ro/}{lg.ccpr.ro}

\section{Forme Canonice}

\renewcommand{\arraystretch}{1.1}

\begin{table}[h!]
    \centering
    \begin{tabular}{|c|c|c|c|c|c|c|}
        \hline
        \# & A & B & C & D & $FCD,\sum,n$ & $FCC,\Pi,m$ \\ \hline
        0 & 0 & 0 & 0 & 0 & $\bar{A}\bar{B}\bar{C}\bar{D}$ & $A+B+C+D$ \\ \hline
        1 & 0 & 0 & 0 & 1 & $\bar{A}\bar{B}\bar{C}D$ & $A+B+C+\bar{D}$ \\ \hline
        2 & 0 & 0 & 1 & 0 & $\bar{A}\bar{B}C\bar{D}$ & $A+B+\bar{C}+D$ \\ \hline
        3 & 0 & 0 & 1 & 1 & $\bar{A}\bar{B}CD$ & $A+B+\bar{C}+\bar{D}$ \\ \hline
        4 & 0 & 1 & 0 & 0 & $\bar{A}B\bar{C}\bar{D}$ & $A+\bar{B}+C+D$ \\ \hline
        5 & 0 & 1 & 0 & 1 & $\bar{A}B\bar{C}D$ & $A+\bar{B}+C+\bar{D}$ \\ \hline
        6 & 0 & 1 & 1 & 0 & $\bar{A}BC\bar{D}$ & $A+\bar{B}+\bar{C}+D$ \\ \hline
        7 & 0 & 1 & 1 & 1 & $\bar{A}BCD$ & $A+\bar{B}+\bar{C}+\bar{D}$ \\ \hline
        8 & 1 & 0 & 0 & 0 & $A\bar{B}\bar{C}\bar{D}$ & $\bar{A}+B+C+D$ \\ \hline
        9 & 1 & 0 & 0 & 1 & $A\bar{B}\bar{C}D$ & $\bar{A}+B+C\bar{D}$ \\ \hline
        10 & 1 & 0 & 1 & 0 & $A\bar{B}C\bar{D}$ & $\bar{A}+B+\bar{C}+D$ \\ \hline
        11 & 1 & 0 & 1 & 1 & $A\bar{B}CD$ & $\bar{A}+B+\bar{C}+\bar{D}$ \\ \hline
        12 & 1 & 1 & 0 & 0 & $AB\bar{C}\bar{D}$ & $\bar{A}+\bar{B}+C+D$ \\ \hline
        13 & 1 & 1 & 0 & 1 & $AB\bar{C}D$ & $\bar{A}+\bar{B}+C+\bar{D}$ \\ \hline
        14 & 1 & 1 & 1 & 0 & $ABC\bar{D}$ & $\bar{A}+\bar{B}+\bar{C}+D$ \\ \hline
        15 & 1 & 1 & 1 & 1 & $ABCD$ & $\bar{A}+\bar{B}+\bar{C}+\bar{D}$ \\ \hline
    \end{tabular}
\end{table}

\begin{center}
    \textbf{Exerciții}
\end{center}

\begin{figure}[h!]
    \begin{minipage}{0.6\textwidth}
        \textbf{Exercițiul 1:\\}
        $y: 2^2 \rightarrow 2^1$;
        $y = A(A + \bar{B})$\\
        \textbf{Rezolvare:}
        $FCD_{y}=\sum(2,3)=n(2,3)=A\bar{B}+AB$\\
        $ FCC_{y}=\Pi(0,1)=m(0,1)=(A+B)(A+\bar{B}) $\\
        $ y= A\bar{B}+AB=A(\bar{B}+B)=A\times1=A$\\
        $y=(A+B)(A+\bar{B})=A^2+A\bar{B}+BA+B\bar{B}=A+A\bar{B}+AB+0=A(1+B+\bar{B})=A$\\
    \end{minipage}
    \hfill
    \begin{minipage}{0.35\textwidth}
        \begin{tabular}{|c|c|c|c|c|}
            \hline
            A & B & $\bar{B}$ & $A+\bar{B}$ & y \\ \hline
            0 & 0 & 1 & 1 & 0 \\ \hline
            0 & 1 & 0 & 0 & 0 \\ \hline
            1 & 0 & 1 & 1 & 1 \\ \hline
            1 & 1 & 0 & 1 & 1 \\ \hline
        \end{tabular}
    \end{minipage}
\end{figure}


\begin{figure}[h!]
    \begin{minipage}{0.6\textwidth}
        \textbf{Exercițiul 2:\\}
        $f,g:2^2\rightarrow2^1$\\
        $f=\bar{AB}$ ; $g=\bar{A}+\bar{B}$\\
        $f=g?$\\
        \textbf{Rezolvare:}
        $FCD_{y}=\sum(0,1,2)=n(0,1,2)=\bar{A}\bar{B}+\bar{A}B+A\bar{B}$\\
        $FCC_{y}=\Pi(3)=m(3)=\bar{A}+\bar{B}$\\
        Din tabel se observă că f=g\\
    \end{minipage}
    \hfill
    \begin{minipage}{0.4\textwidth}
        \begin{tabular}{|c|c|c|c|c|c|c|c|c|}
            \hline
            \# & A & B & $\bar{A}$ & $\bar{B}$ & AB & $\bar{AB}$ & f & g \\ \hline
            0 & 0 & 0 & 1 & 1 & 0 & 1 & 1 & 1\\ \hline
            1 & 0 & 1 & 1 & 0 & 0 & 1 & 1 & 1\\ \hline
            2 & 1 & 0 & 0 & 1 & 0 & 1 & 1 & 1\\ \hline
            3 & 1 & 1 & 0 & 0 & 1 & 0 & 0 & 0\\ \hline
        \end{tabular}
    \end{minipage}
\end{figure}

\begin{figure}[h!]
    \begin{minipage}{0.6\textwidth}
        \textbf{Exercițiul 3:\\}
        $f,g:2^2\rightarrow2^1$\\
        $f=\bar{A+B}$ ; $g=\bar{A}\bar{B}$\\
        $f=g?$\\
        \textbf{Rezolvare:}
        $FCD_{y}=\sum(0)=n(0)=\bar{A}\bar{B}$\\
        $FCC_{y}=\Pi(1,2,3)=m(1,2,3)$\\
        $=(A+\bar{B})(\bar{A}+B)(\bar{A}+\bar{B})$\\
        Din tabel se observă că f=g\\
    \end{minipage}
    \hfill
    \begin{minipage}{0.4\textwidth}
        \begin{tabular}{|c|c|c|c|c|c|c|c|c|}
            \hline
            \# & A & B & $\bar{A}$ & $\bar{B}$ & AB & $\bar{AB}$ & f & g \\ \hline
            0 & 0 & 0 & 1 & 1 & 0 & 1 & 1 & 1\\ \hline
            1 & 0 & 1 & 1 & 0 & 0 & 1 & 1 & 1\\ \hline
            2 & 1 & 0 & 0 & 1 & 0 & 1 & 1 & 1\\ \hline
            3 & 1 & 1 & 0 & 0 & 1 & 0 & 0 & 0\\ \hline
        \end{tabular}
    \end{minipage}
\end{figure}

\begin{figure}[h!]
    \begin{minipage}{0.7\textwidth}
        \textbf{Exercițiul 4:\\}
        $y:2^3\rightarrow2^1$\\
        Se dă tabelul\\
        \textbf{Rezolvare:}
        $FCD_{y}=\sum(1,2,5,6) $\\
        $=(\bar{A}\bar{B}C)+(\bar{A}B\bar{C})+ (A\bar{B}C)+(AB\bar{C})$\\
        $FCC_{y}=\Pi(0,3,4,7)$\\
        $=(A+B+C)(A+\bar{B}+\bar{C})(\bar{A}+B+C)(\bar{A}+\bar{B}+\bar{C})$\\
        \begin{enumerate}[label=(\alph*)]
            \item {
                $y=\bar{A}(\bar{B}C+B\bar{C})+A(\bar{B}C+B\bar{C})$\\
                $ = (\bar{A}+A)(\bar{B}C+B\bar{C})=(\bar{B}C+B\bar{C})$\\
                $ = B\bigoplus C$
            }
            \item {
                $y=(A+B+C)(A+\bar{B}+\bar{C})(\bar{A}+B+C)(\bar{A}+\bar{B}+\bar{C})$\\
                $ =(AA+A\bar{B}+A\bar{C}+AB+B\bar{B}+B\bar{C}+AC+\bar{B}C+C\bar{C})(\bar{A}+B+C)(\bar{A}+\bar{B}+\bar{C})$\\
                $ =(A+A(\bar{B}+B)+A(\bar{C}+C)+B\bar{C}+\bar{B}C)(\bar{A}+B+C)(\bar{A}+\bar{B}+\bar{C})$
                $ =(A(1+\bar{B}+B)+A(\bar{C}+C)+ B\bigoplus C)(\bar{A}+B+C)(\bar{A}+B+C)(\bar{A}+\bar{B}+\bar{C})$
                $ =(A+A+B\bigoplus C)(\bar{A}+B+C)(\bar{A}+\bar{B}+\bar{C})$
                $ =(A+B\bigoplus C)(\bar{A}\bar{A}+\bar{A}\bar{B}+\bar{A}\bar{C}+B\bar{A}+B\bar{B}+B\bar{C}+C\bar{A}+C\bar{B}+C\bar{C})$
                $ =(A+B\bigoplus C)(\bar{A}(\bar{B}+\bar{C}+1+B+C)+B\bar{C}+C\bar{B})$
                $ =(A+B\bigoplus C)(\bar{A}+B\bigoplus C)$
                $ =A\bar{A}+A(B\bigoplus C)+\bar{A}(B\bigoplus C)+(B\bar{C}+\bar{B}C)(B\bar{C}+\bar{B}C)$
                $ =0+(B\bigoplus C)(A+\bar{A})+B^2C^2+B\bar{B}C\bar{C}+\bar{B}B\bar{C}C+B^2C^2$
                $ =B\bigoplus C +B\bar{C}+\bar{B}C$
                $ =B\bigoplus C + B\bigoplus C$
                $ =B\bigoplus C$
            }
        \end{enumerate}
    \end{minipage}
    \hfill
    \begin{minipage}{0.2\textwidth}
        \begin{tabular}{|c|c|c|c|c|}
            \hline
            \# & A & B & C & y \\ \hline
            0  & 0 & 0 & 0 & 0 \\ \hline
            1  & 0 & 0 & 1 & 1 \\ \hline
            2  & 0 & 1 & 0 & 1 \\ \hline
            3  & 0 & 1 & 1 & 0 \\ \hline
            4  & 1 & 0 & 0 & 0 \\ \hline
            5  & 1 & 0 & 1 & 1 \\ \hline
            6  & 1 & 1 & 0 & 1 \\ \hline
            7  & 1 & 1 & 1 & 0 \\ \hline
        \end{tabular}
    \end{minipage}
\end{figure}

\begin{figure}[h!]
    \begin{minipage}{0.6\textwidth}
        \textbf{Exercițiul 5:\\}
        $y:2^4\rightarrow2^1$\\
        $y=\sum(0,2,5,7,8,10,13,15)$\\
        $y=\Pi(1,3,4,6,9,11,12,14)$\\
        \textbf{Rezolvare:\\}
        $FCD_{y}=\bar{A}\bar{B}\bar{C}\bar{D}+ \bar{A}\bar{B}C\bar{D}+\bar{A}B\bar{C}D+\bar{A}BCD+A\bar{B}\bar{C}\bar{D}+A\bar{B}C\bar{D}+AB\bar{C}D+ABCD$\\
        $FCC_{y}=(A+B+C+\bar{D})(A+B+\bar{C}+\bar{D})(A+\bar{B}+C+D)(A+\bar{B}+\bar{C}+D)(\bar{A}+B+C+\bar{D})(\bar{A}+B+\bar{C}+\bar{D})(\bar{A}+\bar{B}+\bar{C}+D)$
    \end{minipage}
    \hfill
    \begin{minipage}{0.3\textwidth}
        \begin{tabular}{|c|c|c|c|c|c|}
            \hline
            \# & A & B & C & D & y \\ \hline
            0   & 0 & 0 & 0 & 0 & 1 \\ \hline
            1   & 0 & 0 & 0 & 1 & 0 \\ \hline
            2   & 0 & 0 & 1 & 0 & 1 \\ \hline
            3   & 0 & 0 & 1 & 1 & 0 \\ \hline
            4   & 0 & 1 & 0 & 0 & 0 \\ \hline
            5   & 0 & 1 & 0 & 1 & 1 \\ \hline
            6   & 0 & 1 & 1 & 0 & 0 \\ \hline
            7   & 0 & 1 & 1 & 1 & 1 \\ \hline
            8   & 1 & 0 & 0 & 0 & 1 \\ \hline
            9   & 1 & 0 & 0 & 1 & 0 \\ \hline
            10  & 1 & 0 & 1 & 0 & 1 \\ \hline
            11  & 1 & 0 & 1 & 1 & 0 \\ \hline
            12  & 1 & 1 & 0 & 0 & 0 \\ \hline
            13  & 1 & 1 & 0 & 1 & 1 \\ \hline
            14  & 1 & 1 & 1 & 0 & 0 \\ \hline
            15  & 1 & 1 & 1 & 1 & 1 \\ \hline
        \end{tabular}
    \end{minipage}
\end{figure}

\begin{figure}[!h]
    \begin{minipage}{0.6\textwidth}
        \textbf{Exercițiul 5 B:\\}
        $y=\bar{A}\bar{B}\bar{C}\bar{D}+ \bar{A}\bar{B}C\bar{D}+\bar{A}B\bar{C}D+\bar{A}BCD+A\bar{B}\bar{C}\bar{D}+A\bar{B}C\bar{D}+AB\bar{C}D+ABCD$\\
        $ =\bar{B}\bar{D}(\bar{A}\bar{C}+\bar{A}C+A\bar{C}+AC)+BD(\bar{A}\bar{C}+\bar{A}C+A\bar{C}+AC)$\\
        $ =(A\bar{C}+\bar{A}C+A\bar{C}+AC)(\bar{B}\bar{D}+BD)$\\
        $ =(\bar{A}(\bar{C}+C)+A(\bar{C}+C))(\bar{B}\bar{D}+BD)$\\
        $ =(\bar{A}+A)(\bar{B}\bar{D}+BD)=\bar{B}\bar{D}+BD$\\
        $ =\bar{B\bigoplus D}$\\
    \end{minipage}
    \hfill
    \begin{minipage}{0.4\textwidth}
        \begin{tabular}{|c|c|c|c|c|c|c|c|c|}
            \hline
            B & D & $\bar{B}\bar{D}+BD$ \\ \hline
            0 & 0 &  1+0=1\\ \hline
            0 & 1 &  0+0=0\\ \hline
            1 & 0 &  0+0=0\\ \hline
            1 & 1 &  0+1=1\\ \hline
        \end{tabular}
    \end{minipage}
\end{figure}

\end{document}